more samples

Test/civl/async/2pc.bpl
@@ -20,7 +20,7 @@ type {:datatype} {:linear "pair"} Pair;
 function {:constructor} Pair (xid: Xid, mid: Mid) : Pair;
 
 function {:inline} pair (xid: Xid, mid: Mid, p: Pair) : bool
-{ p == Pair(xid, mid) && participantMid(mid#Pair(p)) }
+{ p == Pair(xid, mid) && participantMid(p->mid) }
 
 // Transaction State
 type MState = int;
@@ -131,7 +131,7 @@ function {:inline} Inv_8 (state: GState, B: [Pair]bool, votes: [Xid]int) : bool
   && SetInv(B)
   && (forall xid: Xid :: VotesEqCoordinatorState(votes, state, xid))
   && (forall xid: Xid :: votes[xid] == -1 || votes[xid] == card(B, xid))
-  && (forall p: Pair :: B[p] && votes[xid#Pair(p)] != -1 ==> UndecidedOrCommitted(state[xid#Pair(p)][mid#Pair(p)]))
+  && (forall p: Pair :: B[p] && votes[p->xid] != -1 ==> UndecidedOrCommitted(state[p->xid][p->mid]))
 }
 
 function {:inline} Inv_9 (state: GState, B: [Pair]bool, xid: Xid) : bool
@@ -233,8 +233,8 @@ Coordinator_TransactionReq () returns (xid: Xid)
   while (i <= numParticipants)
   invariant {:cooperates} {:layer 8,9,10} true;
   invariant {:layer 8} Inv_8(state, B, votes);
-  invariant {:layer 8,10} pairs == (lambda p: Pair :: pair(xid, mid#Pair(p), p) && i <= mid#Pair(p));
-  invariant {:layer 8} votes[xid] == -1 || (forall p: Pair :: pairs[p] ==> UndecidedOrCommitted(state[xid][mid#Pair(p)]));
+  invariant {:layer 8,10} pairs == (lambda p: Pair :: pair(xid, p->mid, p) && i <= p->mid);
+  invariant {:layer 8} votes[xid] == -1 || (forall p: Pair :: pairs[p] ==> UndecidedOrCommitted(state[xid][p->mid]));
   invariant {:layer 9} Inv_9(state, B, xid);
   invariant {:layer 10} gConsistent(state);
   invariant {:layer 10} ExistsMonotoneExtension(snapshot, state, xid);
@@ -433,7 +433,7 @@ modifies UnallocatedXids;
 {
   assume UnallocatedXids[xid];
   assume state[xid] == (lambda j: Mid :: UNDECIDED());
-  pairs := (lambda p: Pair :: pair(xid, mid#Pair(p), p));
+  pairs := (lambda p: Pair :: pair(xid, p->mid, p));
   UnallocatedXids[xid] := false;
 }
 
@@ -449,7 +449,7 @@ procedure {:both} {:layer 8,10} atomic_TransferPair (xid: Xid, mid: Mid, {:linea
 
 function {:inline} {:linear "pair"} XidSetCollector(xids: [Xid]bool) : [Pair]bool
 {
-  (lambda p: Pair :: xids[xid#Pair(p)])
+  (lambda p: Pair :: xids[p->xid])
 }
 
 // ############################################################################
@@ -458,9 +458,9 @@ function {:inline} {:linear "pair"} XidSetCollector(xids: [Xid]bool) : [Pair]boo
 function card(pairs: [Pair]bool, xid: Xid) : int;
 
 procedure {:lemma} Lemma_add_to_set (set: [Pair]bool, pair: Pair);
-requires participantMid(mid#Pair(pair));
+requires participantMid(pair->mid);
 requires !set[pair];
-ensures (forall xid: Xid :: card(set[pair := true], xid) == (if xid == xid#Pair(pair) then card(set, xid) + 1 else card(set, xid)));
+ensures (forall xid: Xid :: card(set[pair := true], xid) == (if xid == pair->xid then card(set, xid) + 1 else card(set, xid)));
 
 procedure {:lemma} Lemma_all_in_set (set: [Pair]bool, xid: Xid);
 requires SetInv(set);
